<?xml version="1.0"?>
<rdf:RDF xmlns="https://bdlweb.phil.uni-erlangen.de/RCxn/ontologies/rcxn#"
     xml:base="https://bdlweb.phil.uni-erlangen.de/RCxn/ontologies/rcxn"
     xmlns:owl="http://www.w3.org/2002/07/owl#"
     xmlns:rdf="http://www.w3.org/1999/02/22-rdf-syntax-ns#"
     xmlns:xml="http://www.w3.org/XML/1998/namespace"
     xmlns:xsd="http://www.w3.org/2001/XMLSchema#"
     xmlns:rdfs="http://www.w3.org/2000/01/rdf-schema#"
     xmlns:rsrch="https://bdlweb.phil.uni-erlangen.de/RCxn/ontologies/rsrch#">
    <owl:Ontology rdf:about="https://bdlweb.phil.uni-erlangen.de/RCxn/ontologies/rcxn"/>
    


    <!-- 
    ///////////////////////////////////////////////////////////////////////////////////////
    //
    // Object Properties
    //
    ///////////////////////////////////////////////////////////////////////////////////////
     -->

    


    <!-- http://purl.org/olia/olia.owl#hasSemanticRole -->

    <owl:ObjectProperty rdf:about="http://purl.org/olia/olia.owl#hasSemanticRole">
        <owl:equivalentProperty rdf:resource="https://bdlweb.phil.uni-erlangen.de/RCxn/ontologies/rcxn#hasSemanticRole"/>
    </owl:ObjectProperty>
    


    <!-- http://www.w3.org/2002/07/owl#topObjectProperty -->

    <rdf:Description rdf:about="http://www.w3.org/2002/07/owl#topObjectProperty">
        <rdfs:domain rdf:resource="https://bdlweb.phil.uni-erlangen.de/RCxn/ontologies/rcxn#Construction"/>
    </rdf:Description>
    


    <!-- https://bdlweb.phil.uni-erlangen.de/RCxn/ontologies/rcxn#annotator -->

    <owl:ObjectProperty rdf:about="https://bdlweb.phil.uni-erlangen.de/RCxn/ontologies/rcxn#annotator">
        <rdfs:subPropertyOf rdf:resource="http://www.w3.org/2002/07/owl#topObjectProperty"/>
        <rdfs:domain rdf:resource="https://bdlweb.phil.uni-erlangen.de/RCxn/ontologies/rcxn#Metadata"/>
        <rdfs:range rdf:resource="https://bdlweb.phil.uni-erlangen.de/RCxn/ontologies/rsrch#Member"/>
        <rdfs:comment xml:lang="en">Relates a construction entry&apos;s metadata to the person who created it.</rdfs:comment>
        <rdfs:label xml:lang="en">Annotator</rdfs:label>
    </owl:ObjectProperty>
    


    <!-- https://bdlweb.phil.uni-erlangen.de/RCxn/ontologies/rcxn#creationDate -->

    <owl:ObjectProperty rdf:about="https://bdlweb.phil.uni-erlangen.de/RCxn/ontologies/rcxn#creationDate">
        <rdfs:subPropertyOf rdf:resource="http://www.w3.org/2002/07/owl#topObjectProperty"/>
        <rdfs:domain rdf:resource="https://bdlweb.phil.uni-erlangen.de/RCxn/ontologies/rcxn#Metadata"/>
        <rdfs:range>
            <owl:Restriction>
                <owl:onProperty rdf:resource="http://www.w3.org/2002/07/owl#topDataProperty"/>
                <owl:allValuesFrom rdf:resource="http://www.w3.org/2001/XMLSchema#dateTime"/>
            </owl:Restriction>
        </rdfs:range>
        <rdfs:comment xml:lang="en">Indicates the date where the construction entry was created and links it to the construction’s metadata.</rdfs:comment>
        <rdfs:label xml:lang="en">Creation date</rdfs:label>
    </owl:ObjectProperty>
    


    <!-- https://bdlweb.phil.uni-erlangen.de/RCxn/ontologies/rcxn#elementOf -->

    <owl:ObjectProperty rdf:about="https://bdlweb.phil.uni-erlangen.de/RCxn/ontologies/rcxn#elementOf">
        <rdfs:domain rdf:resource="https://bdlweb.phil.uni-erlangen.de/RCxn/ontologies/rcxn#Construction"/>
        <rdfs:range rdf:resource="https://bdlweb.phil.uni-erlangen.de/RCxn/ontologies/rcxn#Construction"/>
        <rdfs:comment xml:lang="en">Relates a construction to the constructions that it is a part of. If the form of one construction element of A is identified as B (property hasSyntacticForm), then B is an element of B.</rdfs:comment>
        <rdfs:label xml:lang="en">Construction Element of</rdfs:label>
    </owl:ObjectProperty>
    


    <!-- https://bdlweb.phil.uni-erlangen.de/RCxn/ontologies/rcxn#hasConstructionMeaning -->

    <owl:ObjectProperty rdf:about="https://bdlweb.phil.uni-erlangen.de/RCxn/ontologies/rcxn#hasConstructionMeaning">
        <rdfs:domain rdf:resource="https://bdlweb.phil.uni-erlangen.de/RCxn/ontologies/rcxn#Construction"/>
        <rdfs:range rdf:resource="https://bdlweb.phil.uni-erlangen.de/RCxn/ontologies/rcxn#ConstructionMeaning"/>
        <rdfs:comment xml:lang="en">Property that relates a construction to its meaning component (an object of type ConstructionMeaning).</rdfs:comment>
    </owl:ObjectProperty>
    


    <!-- https://bdlweb.phil.uni-erlangen.de/RCxn/ontologies/rcxn#hasIS -->

    <owl:ObjectProperty rdf:about="https://bdlweb.phil.uni-erlangen.de/RCxn/ontologies/rcxn#hasIS">
        <rdfs:domain rdf:resource="https://bdlweb.phil.uni-erlangen.de/RCxn/ontologies/rcxn#Slot"/>
        <rdfs:range rdf:resource="https://bdlweb.phil.uni-erlangen.de/RCxn/ontologies/rcxn#informationStructure"/>
        <rdfs:comment xml:lang="en">The construction element is part of the Focus or Background / Topic or Comment of the full utterance.</rdfs:comment>
        <rdfs:label xml:lang="en">Information Structure</rdfs:label>
    </owl:ObjectProperty>
    


    <!-- https://bdlweb.phil.uni-erlangen.de/RCxn/ontologies/rcxn#hasMeaning -->

    <owl:ObjectProperty rdf:about="https://bdlweb.phil.uni-erlangen.de/RCxn/ontologies/rcxn#hasMeaning">
        <rdfs:domain rdf:resource="https://bdlweb.phil.uni-erlangen.de/RCxn/ontologies/rcxn#ConstructionMeaning"/>
        <rdfs:range>
            <owl:Restriction>
                <owl:onProperty rdf:resource="http://www.w3.org/2002/07/owl#topDataProperty"/>
                <owl:someValuesFrom rdf:resource="http://www.w3.org/2000/01/rdf-schema#Literal"/>
            </owl:Restriction>
        </rdfs:range>
        <rdfs:comment xml:lang="en">Property that relates the meaning component of a construction to the corresponding plaintext description of this meaning.</rdfs:comment>
        <rdfs:label xml:lang="en">Meaning of the construction</rdfs:label>
    </owl:ObjectProperty>
    


    <!-- https://bdlweb.phil.uni-erlangen.de/RCxn/ontologies/rcxn#hasMetadata -->

    <owl:ObjectProperty rdf:about="https://bdlweb.phil.uni-erlangen.de/RCxn/ontologies/rcxn#hasMetadata">
        <rdfs:domain rdf:resource="https://bdlweb.phil.uni-erlangen.de/RCxn/ontologies/rcxn#Construction"/>
        <rdfs:range rdf:resource="https://bdlweb.phil.uni-erlangen.de/RCxn/ontologies/rcxn#Metadata"/>
        <rdfs:comment xml:lang="en">Relates a construction to its metadata.</rdfs:comment>
    </owl:ObjectProperty>
    


    <!-- https://bdlweb.phil.uni-erlangen.de/RCxn/ontologies/rcxn#hasOtherSemanticContribution -->

    <owl:ObjectProperty rdf:about="https://bdlweb.phil.uni-erlangen.de/RCxn/ontologies/rcxn#hasOtherSemanticContribution">
        <rdfs:subPropertyOf rdf:resource="https://bdlweb.phil.uni-erlangen.de/RCxn/ontologies/rcxn#hasSemanticContribution"/>
        <rdfs:range>
            <owl:Restriction>
                <owl:onProperty rdf:resource="http://www.w3.org/2002/07/owl#topDataProperty"/>
                <owl:someValuesFrom rdf:resource="http://www.w3.org/2000/01/rdf-schema#Literal"/>
            </owl:Restriction>
        </rdfs:range>
        <rdfs:comment xml:lang="en">Describes the meaning of the construction element in the construction that cannot be captured by the semantic roles of the OLiA ontology.</rdfs:comment>
        <rdfs:label xml:lang="en">Semantic contribution</rdfs:label>
    </owl:ObjectProperty>
    


    <!-- https://bdlweb.phil.uni-erlangen.de/RCxn/ontologies/rcxn#hasPhonology -->

    <owl:ObjectProperty rdf:about="https://bdlweb.phil.uni-erlangen.de/RCxn/ontologies/rcxn#hasPhonology">
        <rdfs:domain rdf:resource="https://bdlweb.phil.uni-erlangen.de/RCxn/ontologies/rcxn#SlotForm"/>
        <rdfs:range>
            <owl:Restriction>
                <owl:onProperty rdf:resource="http://www.w3.org/2002/07/owl#topDataProperty"/>
                <owl:someValuesFrom rdf:resource="http://www.w3.org/2000/01/rdf-schema#Literal"/>
            </owl:Restriction>
        </rdfs:range>
        <rdfs:comment xml:lang="en">Phonological form of the construction element.</rdfs:comment>
        <rdfs:label xml:lang="en">Phonology</rdfs:label>
    </owl:ObjectProperty>
    


    <!-- https://bdlweb.phil.uni-erlangen.de/RCxn/ontologies/rcxn#hasRoot -->

    <owl:ObjectProperty rdf:about="https://bdlweb.phil.uni-erlangen.de/RCxn/ontologies/rcxn#hasRoot">
        <rdfs:domain rdf:resource="https://bdlweb.phil.uni-erlangen.de/RCxn/ontologies/rcxn#SlotForm"/>
        <rdfs:range>
            <owl:Restriction>
                <owl:onProperty rdf:resource="http://www.w3.org/2002/07/owl#topDataProperty"/>
                <owl:someValuesFrom rdf:resource="http://www.w3.org/2000/01/rdf-schema#Literal"/>
            </owl:Restriction>
        </rdfs:range>
        <rdfs:comment xml:lang="en">Describes the form of a construction element as based on a certain root.</rdfs:comment>
        <rdfs:label xml:lang="en">Root</rdfs:label>
    </owl:ObjectProperty>
    


    <!-- https://bdlweb.phil.uni-erlangen.de/RCxn/ontologies/rcxn#hasSemanticContribution -->

    <owl:ObjectProperty rdf:about="https://bdlweb.phil.uni-erlangen.de/RCxn/ontologies/rcxn#hasSemanticContribution">
        <rdfs:domain rdf:resource="https://bdlweb.phil.uni-erlangen.de/RCxn/ontologies/rcxn#Slot"/>
        <rdfs:comment xml:lang="en">Describes the meaning (e.g., semantic role) of the construction element in the construction.</rdfs:comment>
    </owl:ObjectProperty>
    


    <!-- https://bdlweb.phil.uni-erlangen.de/RCxn/ontologies/rcxn#hasSemanticProperty -->

    <owl:ObjectProperty rdf:about="https://bdlweb.phil.uni-erlangen.de/RCxn/ontologies/rcxn#hasSemanticProperty">
        <rdfs:domain rdf:resource="https://bdlweb.phil.uni-erlangen.de/RCxn/ontologies/rcxn#Slot"/>
        <rdfs:range>
            <owl:Restriction>
                <owl:onProperty rdf:resource="http://www.w3.org/2002/07/owl#topDataProperty"/>
                <owl:someValuesFrom rdf:resource="http://www.w3.org/2000/01/rdf-schema#Literal"/>
            </owl:Restriction>
        </rdfs:range>
        <rdfs:comment xml:lang="en">Describes any loosely defined semantic category that the construction element (typically a word) should belong to. E.g. “the noun has a generic meaning” or “the verb denotes a destructive event”</rdfs:comment>
        <rdfs:label xml:lang="en">Semantic property</rdfs:label>
    </owl:ObjectProperty>
    


    <!-- https://bdlweb.phil.uni-erlangen.de/RCxn/ontologies/rcxn#hasSemanticRole -->

    <owl:ObjectProperty rdf:about="https://bdlweb.phil.uni-erlangen.de/RCxn/ontologies/rcxn#hasSemanticRole">
        <rdfs:subPropertyOf rdf:resource="https://bdlweb.phil.uni-erlangen.de/RCxn/ontologies/rcxn#hasSemanticContribution"/>
        <rdfs:range rdf:resource="http://purl.org/olia/olia-top.owl#SemanticRole"/>
        <rdfs:comment xml:lang="en">Describes the semantic role of the construction element in the construction. The semantic roles are defined by the OLiA ontology.</rdfs:comment>
        <rdfs:label xml:lang="en">Semantic role</rdfs:label>
    </owl:ObjectProperty>
    


    <!-- https://bdlweb.phil.uni-erlangen.de/RCxn/ontologies/rcxn#hasSlotForm -->

    <owl:ObjectProperty rdf:about="https://bdlweb.phil.uni-erlangen.de/RCxn/ontologies/rcxn#hasSlotForm">
        <rdfs:domain rdf:resource="https://bdlweb.phil.uni-erlangen.de/RCxn/ontologies/rcxn#Slot"/>
        <rdfs:range rdf:resource="https://bdlweb.phil.uni-erlangen.de/RCxn/ontologies/rcxn#SlotForm"/>
        <rdfs:comment xml:lang="en">Relates a construction element to its formal features.</rdfs:comment>
    </owl:ObjectProperty>
    


    <!-- https://bdlweb.phil.uni-erlangen.de/RCxn/ontologies/rcxn#hasSlots -->

    <owl:ObjectProperty rdf:about="https://bdlweb.phil.uni-erlangen.de/RCxn/ontologies/rcxn#hasSlots">
        <rdfs:domain rdf:resource="https://bdlweb.phil.uni-erlangen.de/RCxn/ontologies/rcxn#Construction"/>
        <rdfs:comment xml:lang="en">Relates a construction to the sequence of construction elements that constitutes it.</rdfs:comment>
    </owl:ObjectProperty>
    


    <!-- https://bdlweb.phil.uni-erlangen.de/RCxn/ontologies/rcxn#hasStem -->

    <owl:ObjectProperty rdf:about="https://bdlweb.phil.uni-erlangen.de/RCxn/ontologies/rcxn#hasStem">
        <rdfs:domain rdf:resource="https://bdlweb.phil.uni-erlangen.de/RCxn/ontologies/rcxn#SlotForm"/>
        <rdfs:range>
            <owl:Restriction>
                <owl:onProperty rdf:resource="http://www.w3.org/2002/07/owl#topDataProperty"/>
                <owl:someValuesFrom rdf:resource="http://www.w3.org/2000/01/rdf-schema#Literal"/>
            </owl:Restriction>
        </rdfs:range>
        <rdfs:comment xml:lang="en">Describes the form of a construction element as based on a certain stem or lemma.</rdfs:comment>
        <rdfs:label xml:lang="en">Stem / Lemma</rdfs:label>
    </owl:ObjectProperty>
    


    <!-- https://bdlweb.phil.uni-erlangen.de/RCxn/ontologies/rcxn#hasSurfaceForm -->

    <owl:ObjectProperty rdf:about="https://bdlweb.phil.uni-erlangen.de/RCxn/ontologies/rcxn#hasSurfaceForm">
        <rdfs:domain rdf:resource="https://bdlweb.phil.uni-erlangen.de/RCxn/ontologies/rcxn#SlotForm"/>
        <rdfs:range>
            <owl:Restriction>
                <owl:onProperty rdf:resource="http://www.w3.org/2002/07/owl#topDataProperty"/>
                <owl:someValuesFrom rdf:resource="http://www.w3.org/2000/01/rdf-schema#Literal"/>
            </owl:Restriction>
        </rdfs:range>
        <rdfs:comment xml:lang="en">Describes the form of a construction element as having a specific surface form.</rdfs:comment>
        <rdfs:label xml:lang="en">Surface form</rdfs:label>
    </owl:ObjectProperty>
    


    <!-- https://bdlweb.phil.uni-erlangen.de/RCxn/ontologies/rcxn#hasSyntacticForm -->

    <owl:ObjectProperty rdf:about="https://bdlweb.phil.uni-erlangen.de/RCxn/ontologies/rcxn#hasSyntacticForm">
        <rdfs:domain rdf:resource="https://bdlweb.phil.uni-erlangen.de/RCxn/ontologies/rcxn#SlotForm"/>
        <rdfs:range rdf:resource="https://bdlweb.phil.uni-erlangen.de/RCxn/ontologies/rcxn#Construction"/>
        <rdfs:comment xml:lang="en">Identifies the form of the element with that of a construction: typically, it would be a morphosyntactic category (a type of morpheme, a part of speech, a phrase type, a clause type).</rdfs:comment>
        <rdfs:label xml:lang="en">Syntactic form</rdfs:label>
    </owl:ObjectProperty>
    


    <!-- https://bdlweb.phil.uni-erlangen.de/RCxn/ontologies/rcxn#hasSyntacticFunction -->

    <owl:ObjectProperty rdf:about="https://bdlweb.phil.uni-erlangen.de/RCxn/ontologies/rcxn#hasSyntacticFunction">
        <rdfs:domain rdf:resource="https://bdlweb.phil.uni-erlangen.de/RCxn/ontologies/rcxn#Slot"/>
        <rdfs:range>
            <owl:Restriction>
                <owl:onProperty rdf:resource="http://www.w3.org/2002/07/owl#topDataProperty"/>
                <owl:someValuesFrom rdf:resource="http://www.w3.org/2000/01/rdf-schema#Literal"/>
            </owl:Restriction>
        </rdfs:range>
        <rdfs:comment xml:lang="en">Relates the construction element to its function. Typical functions are “subject”, “complement”, “modifier” etc.</rdfs:comment>
        <rdfs:label xml:lang="en">Syntactic function</rdfs:label>
    </owl:ObjectProperty>
    


    <!-- https://bdlweb.phil.uni-erlangen.de/RCxn/ontologies/rcxn#hasTitle -->

    <owl:ObjectProperty rdf:about="https://bdlweb.phil.uni-erlangen.de/RCxn/ontologies/rcxn#hasTitle">
        <rdfs:subPropertyOf rdf:resource="http://www.w3.org/2002/07/owl#topObjectProperty"/>
        <rdfs:domain rdf:resource="https://bdlweb.phil.uni-erlangen.de/RCxn/ontologies/rcxn#Construction"/>
        <rdfs:range>
            <owl:Restriction>
                <owl:onProperty rdf:resource="http://www.w3.org/2002/07/owl#topDataProperty"/>
                <owl:someValuesFrom rdf:resource="http://www.w3.org/2000/01/rdf-schema#Literal"/>
            </owl:Restriction>
        </rdfs:range>
        <rdfs:comment xml:lang="en">Property that relates a construction to its name.</rdfs:comment>
        <rdfs:label xml:lang="en">Title</rdfs:label>
    </owl:ObjectProperty>
    


    <!-- https://bdlweb.phil.uni-erlangen.de/RCxn/ontologies/rcxn#usesImageSchema -->

    <owl:ObjectProperty rdf:about="https://bdlweb.phil.uni-erlangen.de/RCxn/ontologies/rcxn#usesImageSchema">
        <rdfs:domain rdf:resource="https://bdlweb.phil.uni-erlangen.de/RCxn/ontologies/rcxn#ConstructionMeaning"/>
        <rdfs:range>
            <owl:Restriction>
                <owl:onProperty rdf:resource="http://www.w3.org/2002/07/owl#topDataProperty"/>
                <owl:someValuesFrom rdf:resource="http://www.w3.org/2000/01/rdf-schema#Literal"/>
            </owl:Restriction>
        </rdfs:range>
        <rdfs:comment xml:lang="en">Relates the meaning component of a construction to the cognitive pattern that it is based on (i.e., containment or path) and that helps convey meaning through spatial or experiential metaphors.</rdfs:comment>
        <rdfs:label xml:lang="en">Image-Schema</rdfs:label>
    </owl:ObjectProperty>
    


    <!-- 
    ///////////////////////////////////////////////////////////////////////////////////////
    //
    // Classes
    //
    ///////////////////////////////////////////////////////////////////////////////////////
     -->

    


    <!-- http://purl.org/olia/olia-top.owl#SemanticRole -->

    <owl:Class rdf:about="http://purl.org/olia/olia-top.owl#SemanticRole"/>
    


    <!-- http://purl.org/olia/olia.owl#Focus -->

    <owl:Class rdf:about="http://purl.org/olia/olia.owl#Focus">
        <owl:equivalentClass rdf:resource="https://bdlweb.phil.uni-erlangen.de/RCxn/ontologies/rcxn#Focus"/>
        <rdfs:subClassOf rdf:resource="http://purl.org/olia/olia.owl#PragmaticUnit"/>
    </owl:Class>
    


    <!-- http://purl.org/olia/olia.owl#PragmaticUnit -->

    <owl:Class rdf:about="http://purl.org/olia/olia.owl#PragmaticUnit"/>
    


    <!-- http://purl.org/olia/olia.owl#Topic -->

    <owl:Class rdf:about="http://purl.org/olia/olia.owl#Topic">
        <owl:equivalentClass rdf:resource="https://bdlweb.phil.uni-erlangen.de/RCxn/ontologies/rcxn#Topic"/>
        <rdfs:subClassOf rdf:resource="http://purl.org/olia/olia.owl#PragmaticUnit"/>
    </owl:Class>
    


    <!-- https://bdlweb.phil.uni-erlangen.de/RCxn/ontologies/rcxn#Background -->

    <owl:Class rdf:about="https://bdlweb.phil.uni-erlangen.de/RCxn/ontologies/rcxn#Background">
        <rdfs:subClassOf rdf:resource="https://bdlweb.phil.uni-erlangen.de/RCxn/ontologies/rcxn#informationStructure"/>
        <rdfs:comment xml:lang="en">The Background is in complementary distribution with the Focus. Typically, the background is discourse-given and can be derived from the context of the utterance. It is the not so relevant information of the utterance.</rdfs:comment>
        <rdfs:label xml:lang="en">Background</rdfs:label>
    </owl:Class>
    


    <!-- https://bdlweb.phil.uni-erlangen.de/RCxn/ontologies/rcxn#Construction -->

    <owl:Class rdf:about="https://bdlweb.phil.uni-erlangen.de/RCxn/ontologies/rcxn#Construction">
        <owl:disjointWith rdf:resource="https://bdlweb.phil.uni-erlangen.de/RCxn/ontologies/rcxn#ConstructionMeaning"/>
        <rdfs:comment xml:lang="en">Construction; linguistic sign with a form component and a meaning component. A network of constructions builds a Constructicon.</rdfs:comment>
    </owl:Class>
    


    <!-- https://bdlweb.phil.uni-erlangen.de/RCxn/ontologies/rcxn#ConstructionMeaning -->

    <owl:Class rdf:about="https://bdlweb.phil.uni-erlangen.de/RCxn/ontologies/rcxn#ConstructionMeaning"/>
    


    <!-- https://bdlweb.phil.uni-erlangen.de/RCxn/ontologies/rcxn#Focus -->

    <owl:Class rdf:about="https://bdlweb.phil.uni-erlangen.de/RCxn/ontologies/rcxn#Focus">
        <rdfs:subClassOf rdf:resource="https://bdlweb.phil.uni-erlangen.de/RCxn/ontologies/rcxn#informationStructure"/>
        <rdfs:comment xml:lang="en">Focus indicates the presence of alternatives that are relevant for the interpretation of linguistic expressions. (Féry et al. 2007)

That part of an expression which provides the most relevant information in a particular context as opposed to the (not so relevant) rest of information making up the background of the utterance. Typically, focus on a subexpression indicates that it is selected from possible alternatives that are either implicit or given explicitly, whereas the background can be derived from the context of the utterance. (SFB632 Guidelines)

Foci are classified here according to their discourse function (independently from their structural realization).</rdfs:comment>
        <rdfs:isDefinedBy rdf:resource="http://purl.org/olia/olia.owl#Focus"/>
        <rdfs:label xml:lang="en">Focus</rdfs:label>
    </owl:Class>
    


    <!-- https://bdlweb.phil.uni-erlangen.de/RCxn/ontologies/rcxn#ISComment -->

    <owl:Class rdf:about="https://bdlweb.phil.uni-erlangen.de/RCxn/ontologies/rcxn#ISComment">
        <rdfs:subClassOf rdf:resource="https://bdlweb.phil.uni-erlangen.de/RCxn/ontologies/rcxn#informationStructure"/>
        <rdfs:comment xml:lang="en">The Comment is in complementary distribution with the Topic. It is what is said about the topic, the main predication of the utterance.</rdfs:comment>
        <rdfs:label xml:lang="en">Comment</rdfs:label>
    </owl:Class>
    


    <!-- https://bdlweb.phil.uni-erlangen.de/RCxn/ontologies/rcxn#Metadata -->

    <owl:Class rdf:about="https://bdlweb.phil.uni-erlangen.de/RCxn/ontologies/rcxn#Metadata">
        <rdfs:comment xml:lang="en">Non-linguistic information on the construction entry, such as the persons involved in the creation of the entry or the sources.</rdfs:comment>
    </owl:Class>
    


    <!-- https://bdlweb.phil.uni-erlangen.de/RCxn/ontologies/rcxn#Slot -->

    <owl:Class rdf:about="https://bdlweb.phil.uni-erlangen.de/RCxn/ontologies/rcxn#Slot">
        <rdfs:comment xml:lang="en">Construction elements in the construction. They encompass both slot elements, which are positions where specific lexical items or phrases can be inserted, and lexically defined elements, which are fixed words or phrases that contribute to the construction&apos;s specific form and meaning. In constructicography, construction elements are linked together by &quot;sequential&quot; links.</rdfs:comment>
    </owl:Class>
    


    <!-- https://bdlweb.phil.uni-erlangen.de/RCxn/ontologies/rcxn#SlotForm -->

    <owl:Class rdf:about="https://bdlweb.phil.uni-erlangen.de/RCxn/ontologies/rcxn#SlotForm">
        <rdfs:comment xml:lang="en">Formal features of a construction element.</rdfs:comment>
    </owl:Class>
    


    <!-- https://bdlweb.phil.uni-erlangen.de/RCxn/ontologies/rcxn#SlotMandatory -->

    <owl:Class rdf:about="https://bdlweb.phil.uni-erlangen.de/RCxn/ontologies/rcxn#SlotMandatory">
        <rdfs:subClassOf rdf:resource="https://bdlweb.phil.uni-erlangen.de/RCxn/ontologies/rcxn#Slot"/>
        <owl:disjointWith rdf:resource="https://bdlweb.phil.uni-erlangen.de/RCxn/ontologies/rcxn#SlotOptional"/>
        <rdfs:comment xml:lang="en">Non-optional construction elements that need to be realized.</rdfs:comment>
        <rdfs:label xml:lang="en">Non-optional element</rdfs:label>
    </owl:Class>
    


    <!-- https://bdlweb.phil.uni-erlangen.de/RCxn/ontologies/rcxn#SlotOptional -->

    <owl:Class rdf:about="https://bdlweb.phil.uni-erlangen.de/RCxn/ontologies/rcxn#SlotOptional">
        <rdfs:subClassOf rdf:resource="https://bdlweb.phil.uni-erlangen.de/RCxn/ontologies/rcxn#Slot"/>
        <rdfs:comment xml:lang="en">Optional construction elements; the meaning of the construction is not dependent on its realization.</rdfs:comment>
        <rdfs:label xml:lang="en">Optional element</rdfs:label>
    </owl:Class>
    


    <!-- https://bdlweb.phil.uni-erlangen.de/RCxn/ontologies/rcxn#Topic -->

    <owl:Class rdf:about="https://bdlweb.phil.uni-erlangen.de/RCxn/ontologies/rcxn#Topic">
        <rdfs:subClassOf rdf:resource="https://bdlweb.phil.uni-erlangen.de/RCxn/ontologies/rcxn#informationStructure"/>
        <rdfs:comment xml:lang="en">The topic constituent identifies the entity or set of entities under which the information expressed in the comment constituent should be stored in the CG content.

The notion of topic is best understood as a kind of address or file card which specifies the individual or set about which the remainder of the sentence makes a comment (see Reinhart 1981 for such a concept of topicality). It has no truthconditional effect except that it presupposes the existence of that individual. In this sense, the complement of ‘topic’ is ‘comment,’ which can itself be partitioned into a focused and a backgrounded part. Sentences usually have only one topic, but can also have none, or more than one. Following Jacobs (2001), topics can be aboutness or frame-setting topics, and the means to express a topic in the grammar can be pinpointed rather precisely in terms of which syntactic and intonational preferences the topic displays, at least in an intonation language. However, according to Féry’s theses, none of these properties are definitional for topic. Rather they express preferences as to how a ‘good’ topic has to be realized (see also Jacobs 2001 for a similar view).

(Féry et al. 2007)</rdfs:comment>
        <rdfs:isDefinedBy rdf:resource="http://purl.org/olia/olia.owl#Topic"/>
        <rdfs:label xml:lang="en">Topic</rdfs:label>
    </owl:Class>
    


    <!-- https://bdlweb.phil.uni-erlangen.de/RCxn/ontologies/rcxn#informationStructure -->

    <owl:Class rdf:about="https://bdlweb.phil.uni-erlangen.de/RCxn/ontologies/rcxn#informationStructure"/>
    


    <!-- https://bdlweb.phil.uni-erlangen.de/RCxn/ontologies/rsrch#Member -->

    <owl:Class rdf:about="https://bdlweb.phil.uni-erlangen.de/RCxn/ontologies/rsrch#Member"/>
</rdf:RDF>



<!-- Generated by the OWL API (version 4.5.29.2024-05-13T12:11:03Z) https://github.com/owlcs/owlapi -->

