<?xml version="1.0"?>
<rdf:RDF xmlns="https://bdlweb.phil.uni-erlangen.de/RCxn/ontologies/rcxn#"
     xml:base="https://bdlweb.phil.uni-erlangen.de/RCxn/ontologies/rcxn"
     xmlns:owl="http://www.w3.org/2002/07/owl#"
     xmlns:rdf="http://www.w3.org/1999/02/22-rdf-syntax-ns#"
     xmlns:xml="http://www.w3.org/XML/1998/namespace"
     xmlns:xsd="http://www.w3.org/2001/XMLSchema#"
     xmlns:rdfs="http://www.w3.org/2000/01/rdf-schema#"
     xmlns:rsrch="https://bdlweb.phil.uni-erlangen.de/RCxn/ontologies/rsrch#">
    <owl:Ontology rdf:about="https://bdlweb.phil.uni-erlangen.de/RCxn/ontologies/rcxn"/>
    


    <!-- 
    ///////////////////////////////////////////////////////////////////////////////////////
    //
    // Object Properties
    //
    ///////////////////////////////////////////////////////////////////////////////////////
     -->

    


    <!-- http://www.w3.org/2002/07/owl#topObjectProperty -->

    <rdf:Description rdf:about="http://www.w3.org/2002/07/owl#topObjectProperty">
        <rdfs:domain rdf:resource="https://bdlweb.phil.uni-erlangen.de/RCxn/ontologies/rcxn#Construction"/>
    </rdf:Description>
    


    <!-- https://bdlweb.phil.uni-erlangen.de/RCxn/ontologies/rcxn#annotator -->

    <owl:ObjectProperty rdf:about="https://bdlweb.phil.uni-erlangen.de/RCxn/ontologies/rcxn#annotator">
        <rdfs:subPropertyOf rdf:resource="http://www.w3.org/2002/07/owl#topObjectProperty"/>
        <rdfs:domain rdf:resource="https://bdlweb.phil.uni-erlangen.de/RCxn/ontologies/rcxn#Metadata"/>
        <rdfs:range rdf:resource="https://bdlweb.phil.uni-erlangen.de/RCxn/ontologies/rsrch#Member"/>
        <rdfs:comment xml:lang="en">Relates a construction entry&apos;s metadata to the person who created it.</rdfs:comment>
        <rdfs:label xml:lang="en">Annotator</rdfs:label>
    </owl:ObjectProperty>
    


    <!-- https://bdlweb.phil.uni-erlangen.de/RCxn/ontologies/rcxn#creationDate -->

    <owl:ObjectProperty rdf:about="https://bdlweb.phil.uni-erlangen.de/RCxn/ontologies/rcxn#creationDate">
        <rdfs:subPropertyOf rdf:resource="http://www.w3.org/2002/07/owl#topObjectProperty"/>
        <rdfs:domain rdf:resource="https://bdlweb.phil.uni-erlangen.de/RCxn/ontologies/rcxn#Metadata"/>
        <rdfs:range>
            <owl:Restriction>
                <owl:onProperty rdf:resource="http://www.w3.org/2002/07/owl#topDataProperty"/>
                <owl:allValuesFrom rdf:resource="http://www.w3.org/2001/XMLSchema#dateTime"/>
            </owl:Restriction>
        </rdfs:range>
        <rdfs:comment xml:lang="en">Indicates the date where the construction entry was created and links it to the construction’s metadata.</rdfs:comment>
        <rdfs:label xml:lang="en">Creation date</rdfs:label>
    </owl:ObjectProperty>
    


    <!-- https://bdlweb.phil.uni-erlangen.de/RCxn/ontologies/rcxn#hasConstructionMeaning -->

    <owl:ObjectProperty rdf:about="https://bdlweb.phil.uni-erlangen.de/RCxn/ontologies/rcxn#hasConstructionMeaning">
        <rdfs:domain rdf:resource="https://bdlweb.phil.uni-erlangen.de/RCxn/ontologies/rcxn#Construction"/>
        <rdfs:range rdf:resource="https://bdlweb.phil.uni-erlangen.de/RCxn/ontologies/rcxn#ConstructionMeaning"/>
        <rdfs:comment xml:lang="en">Property that relates a construction to its meaning component (an object of type ConstructionMeaning).</rdfs:comment>
    </owl:ObjectProperty>
    


    <!-- https://bdlweb.phil.uni-erlangen.de/RCxn/ontologies/rcxn#hasMeaning -->

    <owl:ObjectProperty rdf:about="https://bdlweb.phil.uni-erlangen.de/RCxn/ontologies/rcxn#hasMeaning">
        <rdfs:domain rdf:resource="https://bdlweb.phil.uni-erlangen.de/RCxn/ontologies/rcxn#ConstructionMeaning"/>
        <rdfs:range>
            <owl:Restriction>
                <owl:onProperty rdf:resource="http://www.w3.org/2002/07/owl#topDataProperty"/>
                <owl:someValuesFrom rdf:resource="http://www.w3.org/2000/01/rdf-schema#Literal"/>
            </owl:Restriction>
        </rdfs:range>
        <rdfs:comment xml:lang="en">Property that relates the meaning component of a construction to the corresponding plaintext description of this meaning.</rdfs:comment>
        <rdfs:label xml:lang="en">Meaning of the construction</rdfs:label>
    </owl:ObjectProperty>
    


    <!-- https://bdlweb.phil.uni-erlangen.de/RCxn/ontologies/rcxn#hasMetadata -->

    <owl:ObjectProperty rdf:about="https://bdlweb.phil.uni-erlangen.de/RCxn/ontologies/rcxn#hasMetadata">
        <rdfs:domain rdf:resource="https://bdlweb.phil.uni-erlangen.de/RCxn/ontologies/rcxn#Construction"/>
        <rdfs:range rdf:resource="https://bdlweb.phil.uni-erlangen.de/RCxn/ontologies/rcxn#Metadata"/>
        <rdfs:comment xml:lang="en">Relates a construction to its metadata.</rdfs:comment>
    </owl:ObjectProperty>
    


    <!-- https://bdlweb.phil.uni-erlangen.de/RCxn/ontologies/rcxn#hasRoot -->

    <owl:ObjectProperty rdf:about="https://bdlweb.phil.uni-erlangen.de/RCxn/ontologies/rcxn#hasRoot">
        <rdfs:domain rdf:resource="https://bdlweb.phil.uni-erlangen.de/RCxn/ontologies/rcxn#SlotForm"/>
        <rdfs:range>
            <owl:Restriction>
                <owl:onProperty rdf:resource="http://www.w3.org/2002/07/owl#topDataProperty"/>
                <owl:someValuesFrom rdf:resource="http://www.w3.org/2000/01/rdf-schema#Literal"/>
            </owl:Restriction>
        </rdfs:range>
        <rdfs:comment xml:lang="en">Describes the form of a construction element as based on a certain root.</rdfs:comment>
        <rdfs:label xml:lang="en">Root</rdfs:label>
    </owl:ObjectProperty>
    


    <!-- https://bdlweb.phil.uni-erlangen.de/RCxn/ontologies/rcxn#hasSlotForm -->

    <owl:ObjectProperty rdf:about="https://bdlweb.phil.uni-erlangen.de/RCxn/ontologies/rcxn#hasSlotForm">
        <rdfs:domain rdf:resource="https://bdlweb.phil.uni-erlangen.de/RCxn/ontologies/rcxn#Slot"/>
        <rdfs:range rdf:resource="https://bdlweb.phil.uni-erlangen.de/RCxn/ontologies/rcxn#SlotForm"/>
        <rdfs:comment xml:lang="en">Relates a construction element to its formal features.</rdfs:comment>
    </owl:ObjectProperty>
    


    <!-- https://bdlweb.phil.uni-erlangen.de/RCxn/ontologies/rcxn#hasSlots -->

    <owl:ObjectProperty rdf:about="https://bdlweb.phil.uni-erlangen.de/RCxn/ontologies/rcxn#hasSlots">
        <rdfs:domain rdf:resource="https://bdlweb.phil.uni-erlangen.de/RCxn/ontologies/rcxn#Construction"/>
        <rdfs:comment xml:lang="en">Relates a construction to the sequence of construction elements that constitutes it.</rdfs:comment>
    </owl:ObjectProperty>
    


    <!-- https://bdlweb.phil.uni-erlangen.de/RCxn/ontologies/rcxn#hasStem -->

    <owl:ObjectProperty rdf:about="https://bdlweb.phil.uni-erlangen.de/RCxn/ontologies/rcxn#hasStem">
        <rdfs:domain rdf:resource="https://bdlweb.phil.uni-erlangen.de/RCxn/ontologies/rcxn#SlotForm"/>
        <rdfs:range>
            <owl:Restriction>
                <owl:onProperty rdf:resource="http://www.w3.org/2002/07/owl#topDataProperty"/>
                <owl:someValuesFrom rdf:resource="http://www.w3.org/2000/01/rdf-schema#Literal"/>
            </owl:Restriction>
        </rdfs:range>
        <rdfs:comment xml:lang="en">Describes the form of a construction element as based on a certain stem or lemma.</rdfs:comment>
        <rdfs:label xml:lang="en">Stem / Lemma</rdfs:label>
    </owl:ObjectProperty>
    


    <!-- https://bdlweb.phil.uni-erlangen.de/RCxn/ontologies/rcxn#hasSurfaceForm -->

    <owl:ObjectProperty rdf:about="https://bdlweb.phil.uni-erlangen.de/RCxn/ontologies/rcxn#hasSurfaceForm">
        <rdfs:domain rdf:resource="https://bdlweb.phil.uni-erlangen.de/RCxn/ontologies/rcxn#SlotForm"/>
        <rdfs:range>
            <owl:Restriction>
                <owl:onProperty rdf:resource="http://www.w3.org/2002/07/owl#topDataProperty"/>
                <owl:someValuesFrom rdf:resource="http://www.w3.org/2000/01/rdf-schema#Literal"/>
            </owl:Restriction>
        </rdfs:range>
        <rdfs:comment xml:lang="en">Describes the form of a construction element as having a specific surface form.</rdfs:comment>
        <rdfs:label xml:lang="en">Surface form</rdfs:label>
    </owl:ObjectProperty>
    


    <!-- https://bdlweb.phil.uni-erlangen.de/RCxn/ontologies/rcxn#hasSyntacticForm -->

    <owl:ObjectProperty rdf:about="https://bdlweb.phil.uni-erlangen.de/RCxn/ontologies/rcxn#hasSyntacticForm">
        <rdfs:domain rdf:resource="https://bdlweb.phil.uni-erlangen.de/RCxn/ontologies/rcxn#SlotForm"/>
        <rdfs:range>
            <owl:Restriction>
                <owl:onProperty rdf:resource="http://www.w3.org/2002/07/owl#topDataProperty"/>
                <owl:someValuesFrom rdf:resource="http://www.w3.org/2000/01/rdf-schema#Literal"/>
            </owl:Restriction>
        </rdfs:range>
        <rdfs:comment xml:lang="en">Identifies the form of the element with a morphosyntactic category: it may be a type of morpheme (suffix, root, etc.), a part of speech, a phrase, a clause or a larger textual unit.</rdfs:comment>
        <rdfs:label xml:lang="en">Syntactic form</rdfs:label>
    </owl:ObjectProperty>
    


    <!-- https://bdlweb.phil.uni-erlangen.de/RCxn/ontologies/rcxn#hasSyntacticFunction -->

    <owl:ObjectProperty rdf:about="https://bdlweb.phil.uni-erlangen.de/RCxn/ontologies/rcxn#hasSyntacticFunction">
        <rdfs:domain rdf:resource="https://bdlweb.phil.uni-erlangen.de/RCxn/ontologies/rcxn#Slot"/>
        <rdfs:range>
            <owl:Restriction>
                <owl:onProperty rdf:resource="http://www.w3.org/2002/07/owl#topDataProperty"/>
                <owl:someValuesFrom rdf:resource="http://www.w3.org/2000/01/rdf-schema#Literal"/>
            </owl:Restriction>
        </rdfs:range>
        <rdfs:comment xml:lang="en">Relates the construction element to its function. Typical functions are “subject”, “complement”, “modifier” etc.</rdfs:comment>
        <rdfs:label xml:lang="en">Syntactic function</rdfs:label>
    </owl:ObjectProperty>
    


    <!-- https://bdlweb.phil.uni-erlangen.de/RCxn/ontologies/rcxn#hasTitle -->

    <owl:ObjectProperty rdf:about="https://bdlweb.phil.uni-erlangen.de/RCxn/ontologies/rcxn#hasTitle">
        <rdfs:subPropertyOf rdf:resource="http://www.w3.org/2002/07/owl#topObjectProperty"/>
        <rdfs:domain rdf:resource="https://bdlweb.phil.uni-erlangen.de/RCxn/ontologies/rcxn#Construction"/>
        <rdfs:range>
            <owl:Restriction>
                <owl:onProperty rdf:resource="http://www.w3.org/2002/07/owl#topDataProperty"/>
                <owl:someValuesFrom rdf:resource="http://www.w3.org/2000/01/rdf-schema#Literal"/>
            </owl:Restriction>
        </rdfs:range>
        <rdfs:comment xml:lang="en">Property that relates a construction to its name.</rdfs:comment>
        <rdfs:label xml:lang="en">Title</rdfs:label>
    </owl:ObjectProperty>
    


    <!-- https://bdlweb.phil.uni-erlangen.de/RCxn/ontologies/rcxn#usesImageSchema -->

    <owl:ObjectProperty rdf:about="https://bdlweb.phil.uni-erlangen.de/RCxn/ontologies/rcxn#usesImageSchema">
        <rdfs:domain rdf:resource="https://bdlweb.phil.uni-erlangen.de/RCxn/ontologies/rcxn#ConstructionMeaning"/>
        <rdfs:range>
            <owl:Restriction>
                <owl:onProperty rdf:resource="http://www.w3.org/2002/07/owl#topDataProperty"/>
                <owl:someValuesFrom rdf:resource="http://www.w3.org/2000/01/rdf-schema#Literal"/>
            </owl:Restriction>
        </rdfs:range>
        <rdfs:comment xml:lang="en">Relates the meaning component of a construction to the cognitive pattern that it is based on (i.e., containment or path) and that helps convey meaning through spatial or experiential metaphors.</rdfs:comment>
        <rdfs:label xml:lang="en">Image-Schema</rdfs:label>
    </owl:ObjectProperty>
    


    <!-- 
    ///////////////////////////////////////////////////////////////////////////////////////
    //
    // Classes
    //
    ///////////////////////////////////////////////////////////////////////////////////////
     -->

    


    <!-- https://bdlweb.phil.uni-erlangen.de/RCxn/ontologies/rcxn#Construction -->

    <owl:Class rdf:about="https://bdlweb.phil.uni-erlangen.de/RCxn/ontologies/rcxn#Construction">
        <owl:disjointWith rdf:resource="https://bdlweb.phil.uni-erlangen.de/RCxn/ontologies/rcxn#ConstructionMeaning"/>
        <rdfs:comment xml:lang="en">Construction; linguistic sign with a form component and a meaning component. A network of constructions builds a Constructicon.</rdfs:comment>
    </owl:Class>
    


    <!-- https://bdlweb.phil.uni-erlangen.de/RCxn/ontologies/rcxn#ConstructionMeaning -->

    <owl:Class rdf:about="https://bdlweb.phil.uni-erlangen.de/RCxn/ontologies/rcxn#ConstructionMeaning"/>
    


    <!-- https://bdlweb.phil.uni-erlangen.de/RCxn/ontologies/rcxn#Metadata -->

    <owl:Class rdf:about="https://bdlweb.phil.uni-erlangen.de/RCxn/ontologies/rcxn#Metadata">
        <rdfs:comment xml:lang="en">Non-linguistic information on the construction entry, such as the persons involved in the creation of the entry or the sources.</rdfs:comment>
    </owl:Class>
    


    <!-- https://bdlweb.phil.uni-erlangen.de/RCxn/ontologies/rcxn#Slot -->

    <owl:Class rdf:about="https://bdlweb.phil.uni-erlangen.de/RCxn/ontologies/rcxn#Slot">
        <rdfs:comment xml:lang="en">Construction elements in the construction. They encompass both slot elements, which are positions where specific lexical items or phrases can be inserted, and lexically defined elements, which are fixed words or phrases that contribute to the construction&apos;s specific form and meaning. In constructicography, construction elements are linked together by &quot;sequential&quot; links.</rdfs:comment>
    </owl:Class>
    


    <!-- https://bdlweb.phil.uni-erlangen.de/RCxn/ontologies/rcxn#SlotForm -->

    <owl:Class rdf:about="https://bdlweb.phil.uni-erlangen.de/RCxn/ontologies/rcxn#SlotForm">
        <rdfs:comment xml:lang="en">Formal features of a construction element.</rdfs:comment>
    </owl:Class>
    


    <!-- https://bdlweb.phil.uni-erlangen.de/RCxn/ontologies/rcxn#SlotMandatory -->

    <owl:Class rdf:about="https://bdlweb.phil.uni-erlangen.de/RCxn/ontologies/rcxn#SlotMandatory">
        <rdfs:subClassOf rdf:resource="https://bdlweb.phil.uni-erlangen.de/RCxn/ontologies/rcxn#Slot"/>
        <owl:disjointWith rdf:resource="https://bdlweb.phil.uni-erlangen.de/RCxn/ontologies/rcxn#SlotOptional"/>
        <rdfs:comment xml:lang="en">Non-optional construction elements that need to be realized.</rdfs:comment>
    </owl:Class>
    


    <!-- https://bdlweb.phil.uni-erlangen.de/RCxn/ontologies/rcxn#SlotOptional -->

    <owl:Class rdf:about="https://bdlweb.phil.uni-erlangen.de/RCxn/ontologies/rcxn#SlotOptional">
        <rdfs:subClassOf rdf:resource="https://bdlweb.phil.uni-erlangen.de/RCxn/ontologies/rcxn#Slot"/>
        <rdfs:comment xml:lang="en">Optional construction elements; the meaning of the construction is not dependent on its realization.</rdfs:comment>
    </owl:Class>
    


    <!-- https://bdlweb.phil.uni-erlangen.de/RCxn/ontologies/rsrch#Member -->

    <owl:Class rdf:about="https://bdlweb.phil.uni-erlangen.de/RCxn/ontologies/rsrch#Member"/>
</rdf:RDF>



<!-- Generated by the OWL API (version 4.5.26.2023-07-17T20:34:13Z) https://github.com/owlcs/owlapi -->

