<?xml version="1.0"?>
<rdf:RDF xmlns="https://bdlweb.phil.uni-erlangen.de/RCxn/ontologies/rsrch#"
     xml:base="https://bdlweb.phil.uni-erlangen.de/RCxn/ontologies/rsrch"
     xmlns:ns="http://www.w3.org/2003/06/sw-vocab-status/ns#"
     xmlns:owl="http://www.w3.org/2002/07/owl#"
     xmlns:rdf="http://www.w3.org/1999/02/22-rdf-syntax-ns#"
     xmlns:wot="http://xmlns.com/wot/0.1/"
     xmlns:xml="http://www.w3.org/XML/1998/namespace"
     xmlns:xsd="http://www.w3.org/2001/XMLSchema#"
     xmlns:foaf="http://xmlns.com/foaf/0.1/"
     xmlns:rdfs="http://www.w3.org/2000/01/rdf-schema#"
     xmlns:terms="http://purl.org/dc/terms/">
    <owl:Ontology rdf:about="https://bdlweb.phil.uni-erlangen.de/RCxn/ontologies/rsrch"/>
    


    <!-- 
    ///////////////////////////////////////////////////////////////////////////////////////
    //
    // Object Properties
    //
    ///////////////////////////////////////////////////////////////////////////////////////
     -->

    


    <!-- https://bdlweb.phil.uni-erlangen.de/RCxn/ontologies/rsrch#hasFindings -->

    <owl:ObjectProperty rdf:about="https://bdlweb.phil.uni-erlangen.de/RCxn/ontologies/rsrch#hasFindings">
        <rdf:type rdf:resource="http://www.w3.org/2002/07/owl#AsymmetricProperty"/>
        <rdfs:domain rdf:resource="https://bdlweb.phil.uni-erlangen.de/RCxn/ontologies/rsrch#Project"/>
        <rdfs:range rdf:resource="https://bdlweb.phil.uni-erlangen.de/RCxn/ontologies/rsrch#Finding"/>
        <rdfs:comment xml:lang="en">Property that links a research question to the finding(s) answering this research question.</rdfs:comment>
    </owl:ObjectProperty>
    


    <!-- https://bdlweb.phil.uni-erlangen.de/RCxn/ontologies/rsrch#hasResearchQuestion -->

    <owl:ObjectProperty rdf:about="https://bdlweb.phil.uni-erlangen.de/RCxn/ontologies/rsrch#hasResearchQuestion">
        <rdf:type rdf:resource="http://www.w3.org/2002/07/owl#AsymmetricProperty"/>
        <rdf:type rdf:resource="http://www.w3.org/2002/07/owl#TransitiveProperty"/>
        <rdfs:domain rdf:resource="https://bdlweb.phil.uni-erlangen.de/RCxn/ontologies/rsrch#Project"/>
        <rdfs:range rdf:resource="https://bdlweb.phil.uni-erlangen.de/RCxn/ontologies/rsrch#Project"/>
        <rdfs:comment xml:lang="en">Property that breaks down a project or research question and relates it to smaller research questions.</rdfs:comment>
    </owl:ObjectProperty>
    


    <!-- https://bdlweb.phil.uni-erlangen.de/RCxn/ontologies/rsrch#projectName -->

    <owl:ObjectProperty rdf:about="https://bdlweb.phil.uni-erlangen.de/RCxn/ontologies/rsrch#projectName">
        <rdfs:domain rdf:resource="https://bdlweb.phil.uni-erlangen.de/RCxn/ontologies/rsrch#Project"/>
        <rdfs:comment xml:lang="en">Property that relates the URI of a project to its exact label.</rdfs:comment>
    </owl:ObjectProperty>
    


    <!-- 
    ///////////////////////////////////////////////////////////////////////////////////////
    //
    // Classes
    //
    ///////////////////////////////////////////////////////////////////////////////////////
     -->

    


    <!-- http://www.w3.org/2000/10/swap/pim/contact#Person -->

    <owl:Class rdf:about="http://www.w3.org/2000/10/swap/pim/contact#Person"/>
    


    <!-- https://bdlweb.phil.uni-erlangen.de/RCxn/ontologies/rsrch#Finding -->

    <owl:Class rdf:about="https://bdlweb.phil.uni-erlangen.de/RCxn/ontologies/rsrch#Finding">
        <rdfs:comment xml:lang="en">Research on a research question leads to one or several finding(s). They are statements, answers to the research question.</rdfs:comment>
    </owl:Class>
    


    <!-- https://bdlweb.phil.uni-erlangen.de/RCxn/ontologies/rsrch#Member -->

    <owl:Class rdf:about="https://bdlweb.phil.uni-erlangen.de/RCxn/ontologies/rsrch#Member">
        <rdfs:subClassOf rdf:resource="http://www.w3.org/2000/10/swap/pim/contact#Person"/>
        <rdfs:comment>Member of the research group and/or contributors to the Constructicon.</rdfs:comment>
    </owl:Class>
    


    <!-- https://bdlweb.phil.uni-erlangen.de/RCxn/ontologies/rsrch#PI -->

    <owl:Class rdf:about="https://bdlweb.phil.uni-erlangen.de/RCxn/ontologies/rsrch#PI">
        <rdfs:subClassOf rdf:resource="https://bdlweb.phil.uni-erlangen.de/RCxn/ontologies/rsrch#Member"/>
        <owl:disjointWith rdf:resource="https://bdlweb.phil.uni-erlangen.de/RCxn/ontologies/rsrch#Researcher"/>
        <rdfs:comment xml:lang="en">Researchers supervising or otherwise involved in the research project.</rdfs:comment>
    </owl:Class>
    


    <!-- https://bdlweb.phil.uni-erlangen.de/RCxn/ontologies/rsrch#PostDoc -->

    <owl:Class rdf:about="https://bdlweb.phil.uni-erlangen.de/RCxn/ontologies/rsrch#PostDoc">
        <rdfs:subClassOf rdf:resource="https://bdlweb.phil.uni-erlangen.de/RCxn/ontologies/rsrch#Member"/>
        <owl:disjointWith rdf:resource="https://bdlweb.phil.uni-erlangen.de/RCxn/ontologies/rsrch#Researcher"/>
        <rdfs:comment xml:lang="en">Post-doctoral researcher working in the research group.</rdfs:comment>
    </owl:Class>
    


    <!-- https://bdlweb.phil.uni-erlangen.de/RCxn/ontologies/rsrch#Project -->

    <owl:Class rdf:about="https://bdlweb.phil.uni-erlangen.de/RCxn/ontologies/rsrch#Project">
        <rdfs:subClassOf rdf:resource="http://xmlns.com/foaf/0.1/Project"/>
        <rdfs:comment xml:lang="en">A research question, i.e., a concise inquiry that defines the academic focus of a researcher. Within the terminology of the Research Training Group, the main research question of a PhD candidate for their thesis is called a “project”.</rdfs:comment>
    </owl:Class>
    


    <!-- https://bdlweb.phil.uni-erlangen.de/RCxn/ontologies/rsrch#Researcher -->

    <owl:Class rdf:about="https://bdlweb.phil.uni-erlangen.de/RCxn/ontologies/rsrch#Researcher">
        <rdfs:subClassOf rdf:resource="https://bdlweb.phil.uni-erlangen.de/RCxn/ontologies/rsrch#Member"/>
        <rdfs:comment xml:lang="en">PhD student researcher working in the research group.</rdfs:comment>
    </owl:Class>
</rdf:RDF>



<!-- Generated by the OWL API (version 4.5.26.2023-07-17T20:34:13Z) https://github.com/owlcs/owlapi -->

